silveroak-opentitan/aes/Acorn/AddRoundKeyEquivalence.v
@@ -38,12 +38,29 @@ Section Equivalence.
   Local Notation state := (Vector.t (Vector.t byte 4) 4) (only parsing).
   Local Notation key := (Vector.t (Vector.t byte 4) 4) (only parsing).
 
+  Lemma map2_to_flat (f : bool -> bool -> bool) (v1 v2 : state) :
+    Vector.map2 f (to_flat v1) (to_flat v2)
+    = to_flat (Vector.map2 (Vector.map2 (Vector.map2 f)) v1 v2).
+  Proof.
+    cbv [to_flat]. cbv [BigEndian.from_rows BigEndian.from_cols].
+    cbv [BigEndian.from_big_endian_bytes].
+    cbv [BitArithmetic.bytevec_to_bitvec].
+    autorewrite with pull_vector_map.
+    rewrite !map_map2, !map_map.
+    rewrite !map_id_ext
+      by (intros; rewrite BitArithmetic.bitvec_to_byte_to_bitvec; reflexivity).
+    erewrite map2_ext with
+        (f0 := fun a b => BitArithmetic.byte_to_bitvec (BitArithmetic.bitvec_to_byte _))
+      by (intros; rewrite BitArithmetic.bitvec_to_byte_to_bitvec; reflexivity).
+    autorewrite with pull_vector_map. reflexivity.
+  Qed.
+
   Lemma add_round_key_equiv (k : key) (st : state) :
     combinational (add_round_key [k] [st])
-    = [to_cols_bitvecs (AES256.add_round_key (from_cols_bitvecs st)
-                                             (from_cols_bitvecs k))].
+    = [AES256.aes_add_round_key_circuit_spec k st].
   Proof.
-    cbv [AES256.add_round_key
+    cbv [AES256.aes_add_round_key_circuit_spec
+           AES256.add_round_key
            AcornAes.AddRoundKey.add_round_key
            AesSpec.AddRoundKey.add_round_key].
     cbv [xor4x4V xor4xV]. cbv [Bvector.BVxor].
@@ -59,19 +76,9 @@ Section Equivalence.
                    | intros; rewrite xorV_unIdent by congruence;
                      reflexivity ].
         reflexivity. }
-    cbv [to_cols_bitvecs from_cols_bitvecs]. f_equal.
+    f_equal. rewrite map2_to_cols_bits, map2_to_flat.
     autorewrite with conversions.
-    cbn [fst snd]. rewrite map2_map, map_map2.
-    rewrite map2_swap.
-    erewrite map2_ext; [ reflexivity | ].
-    intros. autorewrite with simpl_ident.
-    erewrite map2_ext
-      by (intros; autorewrite with simpl_ident;
-          cbn [fst snd]; reflexivity).
-    cbn [combType].
-    rewrite <-map2_reshape, !reshape_flatten.
-    rewrite map2_swap. apply map2_ext; intros.
-    rewrite map2_swap. apply map2_ext; intros.
-    intros; apply Bool.xorb_comm.
+    do 3 (rewrite map2_swap; apply map2_ext; intros).
+    apply Bool.xorb_comm.
   Qed.
 End Equivalence.
